WIP
WIP

WIP

WIP

WIP

WIP

WIP

Debugging

WIP

WIP

WIP

WIP

WIP

WIP

WIP

WIP

WIP

WIP

WIP

WIP

WIP

WIP

WIP

WIP

WIP

WIP

WIP

WIP

WIP

WIP

WIP

WIP

Add bound_op

WIP

WIP

WIP

copy_bounds, fill_template

WIP

WIP

WIP

Fix bugs in shr

WIP

WIP

copy_bounds, fill_templates

Add LadderStepDisplay

copy_bounds

Add more notations

Copy bounds

Fix bounds

More notations

C code

More notations for fewer casts

Update log, fix shr

Don't insert identity casts

Update log with elimination of identity casts

Remove useless + casts

Remove useless & casts

Update 32-bit ladder step

Various small notation fixes

Add print of 32-bit ladder

Fix binary notation in 32-bit

Update notations

Update MulDisplay

Add display target

Update notations import

Update notations import

Update display target

Add a bunch of C display files

Remove lowercase files

Add MapBounds

Add 41417 MulDisplay

WIP

Add ComputeBounds

WIP

More/better C notations

Some binary things, remove extra notation

Add Java notations

Remove Java

Hopefully better java display targets

Add Java display things

Add more java display

Add src/SpecificGen/GF25519_64Reflective/Reified/LadderStepJavaDisplay.log

Add more java logs

Constant notation fixes

Add comment about Java casts

davidben tells me unsigned short is bigger than uint8_t

More notations fixes

Fix constants in display

Add more java display

Update display

WIP

WIP

Add TODO

Update TODO

Add to TODO

src/Specific/GF25519Reflective/Reified/rebuild-reified.py
@@ -10,22 +10,22 @@ for name, opkind in ([(name, 'BinOp') for name in ('Add', 'Carry_Add', 'Sub', 'C
     extra = ''
     if name in ('Carry_Add', 'Carry_Sub', 'Mul', 'Carry_Opp', 'Pack', 'Unpack', 'Ge_Modulus', 'PreFreeze'):
         extra = r"""Local Obligation Tactic := intros; vm_compute; constructor.
-Program Definition r%(lname)sW_correct_and_bounded
+Program Definition r%(lname)sZ_correct_and_bounded
   := Expr%(uopkind)s_correct_and_bounded
-       r%(lname)sW %(lname)s r%(lname)sZ_sig r%(lname)sW_correct_and_bounded_gen
+       r%(lname)sZ %(lname)s r%(lname)sZ_sig r%(lname)sZ_correct_and_bounded_gen
        _ _.
 """ % locals()
     with open(name.replace('_', '') + '.v', 'w') as f:
-        f.write(r"""Require Import Crypto.Specific.GF25519Reflective.Common%(uopkind)s.
+        f.write(r"""Require Import Crypto.Specific.GF25519Reflective.Common.
 
 Definition r%(lname)sZ_sig : rexpr_%(lopkind)s_sig %(lname)s. Proof. reify_sig. Defined.
-Definition r%(lname)sW := Eval vm_compute in rword_of_Z r%(lname)sZ_sig.
-Lemma r%(lname)sW_correct_and_bounded_gen : correct_and_bounded_genT r%(lname)sW r%(lname)sZ_sig.
+Definition r%(lname)sZ := Eval vm_compute in proj1_sig r%(lname)sZ_sig.
+Lemma r%(lname)sZ_correct_and_bounded_gen : correct_and_bounded_genT r%(lname)sZ r%(lname)sZ_sig.
 Proof. rexpr_correct. Qed.
-Definition r%(lname)s_output_bounds := Eval vm_compute in compute_bounds r%(lname)sW Expr%(uopkind)s_bounds.
+Definition r%(lname)s_output_bounds := Eval vm_compute in compute_bounds r%(lname)sZ Expr%(uopkind)s_bounds.
 %(extra)s
 Local Open Scope string_scope.
-Compute ("%(name)s", compute_bounds_for_display r%(lname)sW Expr%(uopkind)s_bounds).
-Compute ("%(name)s overflows? ", sanity_compute r%(lname)sW Expr%(uopkind)s_bounds).
-Compute ("%(name)s overflows (error if it does)? ", sanity_check r%(lname)sW Expr%(uopkind)s_bounds).
+Compute ("%(name)s", compute_bounds_for_display r%(lname)sZ Expr%(uopkind)s_bounds).
+Compute ("%(name)s overflows? ", sanity_compute r%(lname)sZ Expr%(uopkind)s_bounds).
+Compute ("%(name)s overflows (error if it does)? ", sanity_check r%(lname)sZ Expr%(uopkind)s_bounds).
 """ % locals())
