src/Reflection/ExprInversion.v
@@ -17,11 +17,10 @@ Section language.
   Local Notation interp_flat_type := (interp_flat_type interp_base_type).
   Local Notation Expr := (@Expr base_type_code op).
 
-  Fixpoint codomain (t : type) : flat_type
-    := match t with
-       | Tflat T => T
-       | Arrow src dst => codomain dst
-       end.
+  Definition domain (t : type) : flat_type
+    := match t with Arrow src dst => src end.
+  Definition codomain (t : type) : flat_type
+    := match t with Arrow src dst => dst end.
 
   Section with_var.
     Context {var : base_type_code -> Type}.
@@ -55,10 +54,8 @@ Section language.
          | Pair _ x _ y => Some (x, y)%core
          | _ => None
          end.
-    Definition invert_Abs {A B} (e : expr (Arrow A B)) : var A -> expr B
+    Definition invert_Abs {A B} (e : expr (Arrow A B)) : interp_flat_type_gen var A -> exprf B
       := match e with Abs _ _ f => f end.
-    Definition invert_Return {t} (e : expr (Tflat t)) : exprf t
-      := match e with Return _ v => v end.
 
     Local Ltac t' :=
       repeat first [ intro
@@ -82,7 +79,6 @@ Section language.
         => revert v;
            refine match e with
                   | Abs _ _ _ => _
-                  | Return _ _ => _
                   end
       end;
       t'.
@@ -106,37 +102,31 @@ Section language.
     Lemma invert_Abs_Some {A B e v}
       : @invert_Abs A B e = v -> e = Abs v.
     Proof. t. Defined.
-
-    Lemma invert_Return_Some {t e v}
-      : @invert_Return t e = v -> e = Return v.
-    Proof. t. Qed.
   End with_var.
 
   Lemma interpf_invert_Abs interp_op {A B e} x
-    : Syntax.interp interp_op (@invert_Abs interp_base_type A B e x)
+    : Syntax.interpf interp_op (@invert_Abs interp_base_type A B e x)
       = Syntax.interp interp_op e x.
   Proof.
     refine (match e in expr _ _ t
                   return match t return expr _ _ t -> _ with
                          | Arrow src dst
                            => fun e
-                              => (forall x : interp_base_type src,
-                                     interp _ (invert_Abs e x) = interp _ e x)
-                         | Tflat _ => fun _ => True
+                              => (forall x : interp_flat_type src,
+                                     interpf _ (invert_Abs e x) = interp _ e x)
                          end e with
             | Abs _ _ _ => fun _ => eq_refl
-            | Return _ _ => I
             end x).
   Qed.
 End language.
 
+Global Arguments domain {_} _.
 Global Arguments codomain {_} _.
 Global Arguments invert_Var {_ _ _ _} _.
 Global Arguments invert_Op {_ _ _ _} _.
 Global Arguments invert_LetIn {_ _ _ _} _.
 Global Arguments invert_Pair {_ _ _ _ _} _.
 Global Arguments invert_Abs {_ _ _ _ _} _ _.
-Global Arguments invert_Return {_ _ _ _} _.
 
 Ltac invert_expr_subst_step :=
   match goal with
@@ -153,7 +143,6 @@ Ltac invert_expr_subst_step :=
        apply invert_Abs_Some in H;
        subst f
   | [ H : invert_Abs ?e = _ |- _ ] => apply invert_Abs_Some in H
-  | [ H : invert_Return ?e = _ |- _ ] => apply invert_Return_Some in H
   | _ => progress subst
   end.
 Ltac invert_expr_subst := repeat invert_expr_subst_step.
