src/Reflection/MapCastInterp.v
@@ -1,0 +1,272 @@
+Require Import Crypto.Reflection.Syntax.
+Require Import Crypto.Reflection.Wf.
+Require Import Crypto.Reflection.SmartMap.
+Require Import Crypto.Reflection.ExprInversion.
+Require Import Crypto.Reflection.MapCast.
+Require Import Crypto.Reflection.Relations.
+Require Import Crypto.Reflection.WfProofs.
+Require Import Crypto.Reflection.WfInversion.
+Require Import Crypto.Util.Sigma.
+Require Import Crypto.Util.Prod.
+Require Import Crypto.Util.Option.
+Require Import Crypto.Util.Tactics.BreakMatch.
+Require Import Crypto.Util.Tactics.DestructHead.
+
+Local Open Scope ctype_scope.
+Local Open Scope expr_scope.
+Section language.
+  Context {base_type_code : Type}
+          {interp_base_type1 : base_type_code -> Type}
+          {interp_base_type2 : base_type_code -> Type}
+          {op : flat_type base_type_code -> flat_type base_type_code -> Type}
+          (interp_op1 : forall src dst, op src dst -> interp_flat_type interp_base_type1 src -> interp_flat_type interp_base_type1 dst)
+          (interp_op2 : forall src dst, op src dst -> interp_flat_type interp_base_type2 src -> interp_flat_type interp_base_type2 dst)
+          (failv : forall {var t}, @exprf base_type_code op var (Tbase t))
+          (new_base_type : forall t, interp_base_type2 t -> base_type_code).
+  Local Notation new_flat_type (*: forall t, interp_flat_type interp_base_type2 t -> flat_type base_type_code1*)
+    := (@SmartFlatTypeMap2 _ _ interp_base_type2 (fun t v => Tbase (new_base_type t v))).
+  Context (transfer_op : forall ovar src1 dst1 src2 dst2
+                                (opc1 : op src1 dst1)
+                                (opc2 : op src2 dst2)
+                                args2
+                                (args' : @exprf base_type_code op ovar (@new_flat_type _ (interpf interp_op2 args2))),
+              @exprf base_type_code op ovar (@new_flat_type _ (interpf interp_op2 (Op opc2 args2)))).
+  Context (R' : forall t1 t2, interp_base_type1 t1 -> interp_base_type2 t2 -> Prop).
+  Local Notation Rt t1 t2 x y (*t1 t2 (x : interp_flat_type interp_base_type1 t1) (y : interp_flat_type interp_base_type2 t2)*)
+    := (interp_flat_type_rel_pointwise2_hetero (t1:=t1) (t2:=t2) R' x y).
+  Local Notation R x y := (Rt _ _ x y).
+  Local Notation RTt t1 t2 x y
+    := (interp_type_rel_pointwise2_hetero (t1:=t1) (t2:=t2) R' x y).
+  Local Notation RT x y := (RTt _ _ x y).
+
+  (*Local Notation interp_flat_type_ivarf_wff G a b
+    := (forall t x y,
+           List.In (existT _ t (x, y)%core) (flatten_binding_list a b)
+           -> wff G x y)
+         (only parsing).*)
+  Local Notation interp_flat_type_ivarf_Rb a b
+    := (forall t x y,
+           List.In (existT _ t (x, y)%core) (flatten_binding_list a b)
+           -> Rt _ (Tbase _) (interpf interp_op1 x) y)
+         (only parsing).
+  Local Notation interp_flat_type_ivarf_R a b
+    := (forall t x y,
+           List.In (existT _ t (x, y)%core) (flatten_binding_list a b)
+           -> R (interpf interp_op1 x) y)
+         (only parsing).
+  Local Notation interp_flat_type_ivarf_R2b a b
+    := (forall t1 t2 x y,
+           List.In (existT _ (t1, t2)%core (x, y)%core) (flatten_binding_list2 a b)
+           -> Rt _ (Tbase _) (interpf interp_op1 x) y)
+         (only parsing).
+  Local Notation interp_flat_type_ivarf_R2 a b
+    := (forall t1 t2 x y,
+           List.In (existT _ (t1, t2)%core (x, y)%core) (flatten_binding_list2 a b)
+           -> R (interpf interp_op1 x) y)
+         (only parsing).
+
+  Context (Rinterp_op : forall src dst opc args1 args2,
+              R args1 args2 -> R (interp_op1 src dst opc args1) (interp_op2 src dst opc args2))
+          (Rtransfer_op : forall src dst
+                                 (opc : op src dst)
+                                 args2
+                                 (args' : @exprf base_type_code op interp_base_type1 (@new_flat_type _ (interpf interp_op2 args2))),
+              R (interpf interp_op1 args') (interpf interp_op2 args2)
+              -> R (interpf interp_op1 (transfer_op _ src dst src dst opc opc args2 args'))
+                   (interpf interp_op2 (Op opc args2))).
+
+  Local Notation ivar t := (@exprf base_type_code op interp_base_type1 (Tbase t)) (only parsing).
+  Local Notation ivarf := (fun t => ivar t).
+  Section with_var.
+    Context (transfer_var : forall tx1 tx2 tC1
+                                   (f : interp_flat_type ivarf tx1 -> exprf base_type_code op (var:=interp_base_type1) tC1)
+                                   (v : interp_flat_type ivarf tx2),
+                exprf base_type_code op (var:=interp_base_type1) tC1).
+
+    Context (R_transfer_var
+             : forall tx1 tx1' tx2 tC1 tC2
+                      (f : interp_flat_type ivarf tx1 -> exprf base_type_code op tC1)
+                      (g : interp_flat_type interp_base_type2 tx1' -> interp_flat_type interp_base_type2 tC2)
+                      v1 v2,
+                (forall a,
+                    interp_flat_type_ivarf_R2b a v2
+                    -> R (interpf interp_op1 (f a)) (g v2))
+                -> interp_flat_type_ivarf_R2b v1 v2
+                -> R (interpf interp_op1 (@transfer_var tx1 tx2 tC1 f v1))
+                     (g v2)).
+
+    Local Notation mapf_interp_cast
+      := (@mapf_interp_cast
+            base_type_code base_type_code interp_base_type2
+            op op interp_op2 failv new_base_type
+            transfer_op).
+    Local Notation map_interp_cast
+      := (@map_interp_cast
+            base_type_code base_type_code interp_base_type2
+            op op interp_op2 failv new_base_type
+            transfer_op).
+
+    (* Local *) Hint Resolve <- List.in_app_iff.
+
+    Local Ltac break_t
+      := first [ progress subst
+               | progress inversion_wf
+               | progress invert_expr_subst
+               | progress inversion_sigma
+               | progress inversion_prod
+               | progress destruct_head sig
+               | progress destruct_head sigT
+               | progress destruct_head ex
+               | progress destruct_head and
+               | progress destruct_head prod
+               | progress break_match_hyps ].
+
+    Local Ltac fin_False :=
+      lazymatch goal with
+      | [ H : False |- _ ] => exfalso; assumption
+      end.
+
+    Local Ltac fin_t0 :=
+      solve [ constructor; eauto
+            | eauto
+            | auto
+            | hnf; auto ].
+
+    Local Ltac fin_t1 :=
+      solve [ lazymatch goal with
+              | [ |- R' _ _ _ _ ] => eapply interp_flat_type_rel_pointwise2_hetero_flatten_binding_list2; eauto
+              end ].
+
+    Local Ltac handle_transfer_var_t :=
+      match goal with
+      | [ |- R (interpf _ (transfer_var _ _ _ _ _)) _ ]
+        => apply R_transfer_var
+      | [ |- R (interpf _ (transfer_var _ _ _ _ _)) (interpf ?interp_op (?e _)) ]
+        => apply R_transfer_var with (g := fun v => interpf interp_op (e v))
+      | [ |- R' ?t1 ?t2 (interpf _ (transfer_var ?tx1 ?tx2 ?tC1 (fun x => x) ?v1)) ?v2 ]
+        => apply (R_transfer_var tx1 (Tbase _) tx2 tC1 (Tbase _) (fun x => x) (fun x => x))
+      | [ H : _ |- R (interpf _ (mapf_interp_cast _ _ _)) (interpf _ _) ]
+        => apply H
+      end.
+
+    Local Ltac handle_list_t :=
+      match goal with
+      | _ => progress cbv [LetIn.Let_In duplicate_types] in *
+      | [ H : List.In _ (_ ++ _) |- _ ] => apply List.in_app_or in H
+      | [ H : List.In _ (List.map _ _) |- _ ]
+        => rewrite List.in_map_iff in H
+      | _ => rewrite <- flatten_binding_list_flatten_binding_list2
+      | [ H : appcontext[flatten_binding_list2] |- _ ]
+        => rewrite <- flatten_binding_list_flatten_binding_list2 in H
+      | [ H : context[flatten_binding_list (SmartVarfMap _ _) (SmartVarfMap _ _)] |- _ ]
+        => rewrite flatten_binding_list_SmartVarfMap in H
+      | [ H : context[flatten_binding_list2 (SmartVarfMap _ _) (SmartVarfMap _ _)] |- _ ]
+        => rewrite flatten_binding_list2_SmartVarfMap in H
+      | [ H : context[flatten_binding_list2 (SmartVarfMap _ _) _] |- _ ]
+        => rewrite flatten_binding_list2_SmartVarfMap1 in H
+      | [ H : context[flatten_binding_list2 _ (SmartVarfMap _ _)] |- _ ]
+        => rewrite flatten_binding_list2_SmartVarfMap2 in H
+      | _ => rewrite <- flatten_binding_list_flatten_binding_list2
+      | _ => rewrite List.in_map_iff
+      end.
+
+    Local Ltac wff_t :=
+      match goal with
+      | [ |- wff _ _ _ ] => constructor
+      | [ H : _ |- wff _ (mapf_interp_cast _ _ _) (mapf_interp_cast _ _ _) ]
+        => eapply H; eauto; []; clear H
+      | _ => solve [ eauto using wff_in_impl_Proper ]
+      end.
+
+    Local Ltac misc_t :=
+      match goal with
+      | [ H : _ |- R' _ _ (interpf _ ?x) ?y ]
+        => is_var x; is_var y; apply H
+      | [ |- exists _, _ ]
+        => eexists (existT _ _ _)
+      | [ |- _ /\ _ ] => split
+      end.
+
+    Local Ltac t_step :=
+      first [ intro
+            | fin_False
+            | progress break_t
+            | fin_t0
+            | progress simpl in *
+            | wff_t
+            | handle_list_t
+            | progress destruct_head' or
+            | fin_t1
+            | handle_transfer_var_t
+            | misc_t ].
+
+    Lemma interpf_mapf_interp_cast
+          G
+          (HG : forall t x y,
+              List.In (existT _ t (x, y)%core) G
+              -> R' (new_base_type t y) t
+                    (interpf interp_op1
+                             (transfer_var (Tbase _) (Tbase _) (Tbase _)
+                                           (fun k => k) x))
+                    y)
+          {t1} e1 ebounds
+          (Hwf : wff G e1 ebounds)
+      : R (interpf interp_op1 (@mapf_interp_cast interp_base_type1 transfer_var t1 e1 t1 ebounds))
+          (interpf interp_op2 ebounds).
+    Proof. induction Hwf; repeat t_step. Qed.
+
+    Local Hint Resolve interpf_mapf_interp_cast.
+
+    Lemma interp_map_interp_cast
+          {t1} e1 ebounds
+          args2
+          (Hwf : wf e1 ebounds)
+      : forall v,
+        R v args2
+        -> R (interp interp_op1 (@map_interp_cast interp_base_type1 transfer_var t1 e1 t1 ebounds args2) v)
+             (interp interp_op2 ebounds args2).
+    Proof.
+      destruct Hwf;
+        repeat match goal with
+               | _ => t_step
+               | [ |- R (interpf _ (mapf_interp_cast _ _ _)) (interpf _ _) ]
+                 => eapply interpf_mapf_interp_cast
+               end.
+    Qed.
+  End with_var.
+
+  Section gen.
+    Context (transfer_var : forall ovar tx1 tx2 tC1
+                                   (ivarf := fun t => @exprf base_type_code op ovar (Tbase t))
+                                   (f : interp_flat_type ivarf tx1 -> exprf base_type_code op (var:=ovar) tC1)
+                                   (v : interp_flat_type ivarf tx2),
+                exprf base_type_code op (var:=ovar) tC1).
+    Context (R_transfer_var
+             : forall tx1 tx1' tx2 tC1 tC2
+                      (f : interp_flat_type ivarf tx1 -> exprf base_type_code op tC1)
+                      (g : interp_flat_type interp_base_type2 tx1' -> interp_flat_type interp_base_type2 tC2)
+                      v1 v2,
+                (forall a,
+                    interp_flat_type_ivarf_R2b a v2
+                    -> R (interpf interp_op1 (f a)) (g v2))
+                -> interp_flat_type_ivarf_R2b v1 v2
+                -> R (interpf interp_op1 (@transfer_var _ tx1 tx2 tC1 f v1))
+                     (g v2)).
+
+    Local Notation MapInterpCast
+      := (@MapInterpCast
+            base_type_code interp_base_type2
+            op interp_op2 failv new_base_type
+            transfer_op transfer_var).
+
+    Lemma InterpMapInterpCast
+          {t} e
+          args
+          (Hwf : Wf e)
+      : forall v,
+        R v args
+        -> R (Interp interp_op1 (@MapInterpCast t e args) v)
+             (Interp interp_op2 e args).
+    Proof. apply interp_map_interp_cast; auto. Qed.
+  End gen.
+End language.
