src/Reflection/MapCastWf.v
@@ -1,0 +1,222 @@
+Require Import Crypto.Reflection.Syntax.
+Require Import Crypto.Reflection.Wf.
+Require Import Crypto.Reflection.SmartMap.
+Require Import Crypto.Reflection.ExprInversion.
+Require Import Crypto.Reflection.MapCast.
+Require Import Crypto.Reflection.WfProofs.
+Require Import Crypto.Reflection.WfInversion.
+Require Import Crypto.Util.Sigma.
+Require Import Crypto.Util.Prod.
+Require Import Crypto.Util.Option.
+Require Import Crypto.Util.Tactics.BreakMatch.
+Require Import Crypto.Util.Tactics.DestructHead.
+
+Local Open Scope ctype_scope.
+Local Open Scope expr_scope.
+Section language.
+  Context {base_type_code : Type}
+          {interp_base_type : base_type_code -> Type}
+          {op : flat_type base_type_code -> flat_type base_type_code -> Type}
+          (interp_op2 : forall src dst, op src dst -> interp_flat_type interp_base_type src -> interp_flat_type interp_base_type dst)
+          (failv : forall {var t}, @exprf base_type_code op var (Tbase t))
+          (new_base_type : forall t, interp_base_type t -> base_type_code).
+  Local Notation new_flat_type (*: forall t, interp_flat_type interp_base_type2 t -> flat_type base_type_code1*)
+    := (@SmartFlatTypeMap2 _ _ interp_base_type (fun t v => Tbase (new_base_type t v))).
+  Context (transfer_op : forall ovar src1 dst1 src2 dst2
+                                (opc1 : op src1 dst1)
+                                (opc2 : op src2 dst2)
+                                args2
+                                (args' : @exprf base_type_code op ovar (@new_flat_type _ (interpf interp_op2 args2))),
+              @exprf base_type_code op ovar (@new_flat_type _ (interpf interp_op2 (Op opc2 args2)))).
+
+  Local Notation interp_flat_type_ivarf_wff G a b
+    := (forall t x y,
+           List.In (existT _ t (x, y)%core) (flatten_binding_list a b)
+           -> wff G x y)
+         (only parsing).
+
+  Section with_var.
+    Context {ovar1 ovar2 : base_type_code -> Type}.
+    Local Notation ivar1 t := (@exprf base_type_code op ovar1 (Tbase t)) (only parsing).
+    Local Notation ivar2 t := (@exprf base_type_code op ovar2 (Tbase t)) (only parsing).
+    Local Notation ivarf1 := (fun t => ivar1 t).
+    Local Notation ivarf2 := (fun t => ivar2 t).
+    Context (transfer_var1 : forall tx1 tx2 tC1
+                                    (f : interp_flat_type ivarf1 tx1 -> exprf base_type_code op (var:=ovar1) tC1)
+                                    (v : interp_flat_type ivarf1 tx2),
+                exprf base_type_code op (var:=ovar1) tC1).
+    Context (transfer_var2 : forall tx1 tx2 tC1
+                                    (f : interp_flat_type ivarf2 tx1 -> exprf base_type_code op (var:=ovar2) tC1)
+                                    (v : interp_flat_type ivarf2 tx2),
+                exprf base_type_code op (var:=ovar2) tC1).
+
+    Context (wff_transfer_op
+             : forall G src1 dst1 src2 dst2 opc1 opc2 args2 e1 e2,
+                wff G (var1:=ovar1) (var2:=ovar2) e1 e2
+                -> wff G
+                       (@transfer_op ovar1 src1 dst1 src2 dst2 opc1 opc2 args2 e1)
+                       (@transfer_op ovar2 src1 dst1 src2 dst2 opc1 opc2 args2 e2)).
+    Context (wff_transfer_var
+             : forall G tx1 tx2 tC1 f g v1 v2,
+                (forall a b,
+                    interp_flat_type_ivarf_wff G a b
+                    -> wff G (f a) (g b))
+                -> interp_flat_type_ivarf_wff G v1 v2
+                -> wff G
+                       (@transfer_var1 tx1 tx2 tC1 f v1)
+                       (@transfer_var2 tx1 tx2 tC1 g v2)).
+    Local Notation mapf_interp_cast
+      := (@mapf_interp_cast
+            base_type_code base_type_code interp_base_type
+            op op interp_op2 failv new_base_type
+            transfer_op).
+    Local Notation map_interp_cast
+      := (@map_interp_cast
+            base_type_code base_type_code interp_base_type
+            op op interp_op2 failv new_base_type
+            transfer_op).
+
+    Local Notation G1eTf
+      := (fun t : base_type_code => interp_flat_type ivarf1 (Tbase t) * interp_flat_type ivarf2 (Tbase t))%type.
+    Local Notation G2eTf
+      := (fun t : base_type_code => ovar1 t * ovar2 t)%type.
+    Local Notation GbeTf
+      := (fun t : base_type_code => interp_flat_type ivarf1 (Tbase t) * interp_base_type t)%type.
+
+    (*  Definition Gse_related' {t} (G1e : G1eTf t) (Gbe : GbeTf t) (G2e G2eTf t) : Prop
+    := fst G1e = fst Gbe /\
+
+    := exists (pf1 : projT1 G1e = projT1 G2e
+
+                                         Definition Gse_related (G1e : sigT G1eTf) (G2e : sigT G2eTf) (G3e : sigT G3eTf) : Prop
+    := exists (pf1 : projT1 G1e = projT1 G2e
+                   /\
+
+  Local Notation G3eT
+    := {t : base_type_code &
+            ((interp_flat_type ivarf1 (Tbase t) * interp_flat_type ivarf2 (Tbase t))
+             * (ovar1 t * ovar2 t)
+             * interp_base_type t)%type }.
+  Local Notation G3T
+    := (list G3eT).
+
+  Definition G3e_to_G1e
+
+     *)
+    (* Local *) Hint Resolve <- List.in_app_iff.
+
+    Local Ltac break_t
+      := first [ progress subst
+               | progress inversion_wf
+               | progress invert_expr_subst
+               | progress inversion_sigma
+               | progress inversion_prod
+               | progress destruct_head sig
+               | progress destruct_head sigT
+               | progress destruct_head ex
+               | progress destruct_head and
+               | progress destruct_head prod
+               | progress break_match_hyps ].
+
+    Lemma wff_mapf_interp_cast
+          G1 Gbounds G2
+          (H_G1_G2
+           : forall t x y,
+              List.In (existT _ t (x, y)%core) G1
+              -> wff G2 x y)
+          {t1} e1 e2 ebounds
+          (Hwf_bounds : wff Gbounds e1 ebounds)
+          (Hwf : wff G1 e1 e2)
+      : wff G2
+            (@mapf_interp_cast ovar1 transfer_var1 t1 e1 t1 ebounds)
+            (@mapf_interp_cast ovar2 transfer_var2 t1 e2 t1 ebounds).
+    Proof.
+      revert dependent Gbounds; revert ebounds; revert dependent G2.
+      induction Hwf;
+        repeat match goal with
+               | _ => solve [ exfalso; assumption ]
+               | _ => intro
+               | _ => progress break_t
+               | _ => solve [ constructor; eauto
+                            | eauto
+                            | auto
+                            | hnf; auto ]
+               | _ => progress simpl in *
+               | [ |- wff _ (transfer_var1 _ _ _ _ _) (transfer_var2 _ _ _ _ _) ]
+                 => apply wff_transfer_var
+               | [ H : List.In _ (_ ++ _) |- _ ] => apply List.in_app_or in H
+               | _ => progress destruct_head or
+               | [ |- wff _ _ _ ] => constructor
+               | [ H : _ |- wff _ (mapf_interp_cast _ _ _) (mapf_interp_cast _ _ _) ]
+                 => eapply H; eauto; []; clear H
+               | _ => solve [ eauto using wff_in_impl_Proper ]
+               | [ H : context[flatten_binding_list (SmartVarfMap _ _) (SmartVarfMap _ _)] |- _ ]
+                 => rewrite flatten_binding_list_SmartVarfMap in H
+               | [ H : List.In _ (List.map _ _) |- _ ]
+                 => rewrite List.in_map_iff in H
+               end.
+    Qed.
+
+    Lemma wf_map_interp_cast
+          {t1} e1 e2 ebounds
+          args2
+          (Hwf_bounds : wf e1 ebounds)
+          (Hwf : wf e1 e2)
+      : wf (@map_interp_cast ovar1 transfer_var1 t1 e1 t1 ebounds args2)
+           (@map_interp_cast ovar2 transfer_var2 t1 e2 t1 ebounds args2).
+    Proof.
+      destruct Hwf;
+        repeat match goal with
+               | _ => solve [ constructor; eauto
+                            | eauto using wff_mapf_interp_cast
+                            | exfalso; assumption ]
+               | _ => intro
+               | _ => progress break_t
+               | [ |- wf _ _ ] => constructor
+               | [ |- wff _ (transfer_var1 _ _ _ _ _) (transfer_var2 _ _ _ _ _) ]
+                 => apply wff_transfer_var
+               | [ H : context[flatten_binding_list (SmartVarfMap _ _) (SmartVarfMap _ _)] |- _ ]
+                 => rewrite flatten_binding_list_SmartVarfMap in H
+               | [ H : List.In _ (List.map _ _) |- _ ]
+                 => rewrite List.in_map_iff in H
+               end.
+    Qed.
+  End with_var.
+
+  Section gen.
+    Context (wff_transfer_op
+             : forall ovar1 ovar2 G src1 dst1 src2 dst2 opc1 opc2 args2 e1 e2,
+                wff G (var1:=ovar1) (var2:=ovar2) e1 e2
+                -> wff G
+                       (@transfer_op ovar1 src1 dst1 src2 dst2 opc1 opc2 args2 e1)
+                       (@transfer_op ovar2 src1 dst1 src2 dst2 opc1 opc2 args2 e2)).
+    Context (transfer_var : forall ovar tx1 tx2 tC1
+                                   (ivarf := fun t => @exprf base_type_code op ovar (Tbase t))
+                                   (f : interp_flat_type ivarf tx1 -> exprf base_type_code op (var:=ovar) tC1)
+                                   (v : interp_flat_type ivarf tx2),
+                exprf base_type_code op (var:=ovar) tC1).
+    Context (wff_transfer_var
+             : forall ovar1 ovar2 G tx1 tx2 tC1 f g v1 v2,
+                (forall a b,
+                    interp_flat_type_ivarf_wff G a b
+                    -> wff G (f a) (g b))
+                -> interp_flat_type_ivarf_wff G v1 v2
+                -> wff G
+                       (@transfer_var ovar1 tx1 tx2 tC1 f v1)
+                       (@transfer_var ovar2 tx1 tx2 tC1 g v2)).
+    Local Notation MapInterpCast
+      := (@MapInterpCast
+            base_type_code interp_base_type
+            op interp_op2 failv new_base_type
+            transfer_op transfer_var).
+
+    Lemma WfMapInterpCast
+          {t} e
+          args
+          (Hwf : Wf e)
+      : Wf (@MapInterpCast t e args).
+    Proof.
+      intros ??; apply wf_map_interp_cast; auto.
+    Qed.
+  End gen.
+End language.
