src/Reflection/Z/Interpretations.v
@@ -1,0 +1,368 @@
+(** * Interpretation of PHOAS syntax for expression trees on ℤ *)
+Require Import Coq.ZArith.ZArith.
+Require Import Crypto.Reflection.Z.Syntax.
+Require Import Crypto.Reflection.Syntax.
+Require Import Crypto.Reflection.SmartMap.
+Require Import Crypto.Reflection.ExprInversion.
+Require Import Crypto.Reflection.Equality.
+Require Import Crypto.Reflection.MapCastWithCastOp.
+Require Import Crypto.ModularArithmetic.ModularBaseSystemListZOperations.
+Require Import Crypto.Util.Equality.
+Require Import Crypto.Util.ZUtil.
+Require Import Crypto.Util.Option.
+Require Crypto.Util.Tuple.
+Require Crypto.Util.HList.
+Require Import Crypto.Util.Bool.
+Require Import Crypto.Util.Prod.
+Require Import Crypto.Util.Tactics.
+Require Import Bedrock.Word.
+Require Import Crypto.Util.WordUtil.
+Export Reflection.Syntax.Notations.
+
+Local Notation eta x := (fst x, snd x).
+Local Notation eta3 x := (eta (fst x), snd x).
+Local Notation eta4 x := (eta3 (fst x), snd x).
+
+Module Import Bounds.
+  Record bounds := { lower : Z ; upper : Z }.
+
+  Bind Scope bounds_scope with bounds.
+  Definition t := option bounds. (* TODO?: Separate out the bounds computation from the overflow computation? e.g., have [safety := in_bounds | overflow] and [t := bounds * safety]? *)
+  Bind Scope bounds_scope with t.
+  Local Coercion Z.of_nat : nat >-> Z.
+  (*Definition wordWToBounds (x : WordW.wordW) : t
+    := let v := WordW.wordWToZ x in Some {| lower := v ; upper := v |}.*)
+  Definition SmartBuildBounds (l u : Z)
+    := if ((0 <=? l) (*&& (Z.log2 u <? WordW.bit_width)*))%Z%bool
+       then Some {| lower := l ; upper := u |}
+       else None.
+  Definition t_map1 (f : bounds -> bounds) (x : t)
+    := match x with
+       | Some x
+         => match f x with
+            | Build_bounds l u
+              => SmartBuildBounds l u
+            end
+       | _ => None
+       end%Z.
+  Definition t_map2 (f : bounds -> bounds -> bounds) (x y : t)
+    := match x, y with
+       | Some x, Some y
+         => match f x y with
+            | Build_bounds l u
+              => SmartBuildBounds l u
+            end
+       | _, _ => None
+       end%Z.
+  Definition t_map4 (f : bounds -> bounds -> bounds -> bounds -> bounds) (x y z w : t)
+    := match x, y, z, w with
+       | Some x, Some y, Some z, Some w
+         => match f x y z w with
+            | Build_bounds l u
+              => SmartBuildBounds l u
+            end
+       | _, _, _, _ => None
+       end%Z.
+  Definition add' : bounds -> bounds -> bounds
+    := fun x y => let (lx, ux) := x in let (ly, uy) := y in {| lower := lx + ly ; upper := ux + uy |}.
+  Definition add : t -> t -> t := t_map2 add'.
+  Definition sub' : bounds -> bounds -> bounds
+    := fun x y => let (lx, ux) := x in let (ly, uy) := y in {| lower := lx - uy ; upper := ux - ly |}.
+  Definition sub : t -> t -> t := t_map2 sub'.
+  Definition mul' : bounds -> bounds -> bounds
+    := fun x y => let (lx, ux) := x in let (ly, uy) := y in {| lower := lx * ly ; upper := ux * uy |}.
+  Definition mul : t -> t -> t := t_map2 mul'.
+  Definition shl' : bounds -> bounds -> bounds
+    := fun x y => let (lx, ux) := x in let (ly, uy) := y in {| lower := lx << ly ; upper := ux << uy |}.
+  Definition shl : t -> t -> t := t_map2 shl'.
+  Definition shr' : bounds -> bounds -> bounds
+    := fun x y => let (lx, ux) := x in let (ly, uy) := y in {| lower := lx >> uy ; upper := ux >> ly |}.
+  Definition shr : t -> t -> t := t_map2 shr'.
+  Definition land' : bounds -> bounds -> bounds
+    := fun x y => let (lx, ux) := x in let (ly, uy) := y in {| lower := 0 ; upper := Z.min ux uy |}.
+  Definition land : t -> t -> t := t_map2 land'.
+  Definition lor' : bounds -> bounds -> bounds
+    := fun x y => let (lx, ux) := x in let (ly, uy) := y in
+                                       {| lower := Z.max lx ly;
+                                          upper := 2^(Z.max (Z.log2_up (ux+1)) (Z.log2_up (uy+1))) - 1 |}.
+  Definition lor : t -> t -> t := t_map2 lor'.
+  Definition neg' (int_width : Z) : bounds -> bounds
+    := fun v
+       => let (lb, ub) := v in
+          let might_be_one := ((lb <=? 1) && (1 <=? ub))%Z%bool in
+          let must_be_one := ((lb =? 1) && (ub =? 1))%Z%bool in
+          if must_be_one
+          then {| lower := Z.ones int_width ; upper := Z.ones int_width |}
+          else if might_be_one
+               then {| lower := 0 ; upper := Z.ones int_width |}
+               else {| lower := 0 ; upper := 0 |}.
+  Definition neg (int_width : Z) : t -> t
+    := fun v
+       => if ((0 <=? int_width) (*&& (int_width <=? WordW.bit_width)*))%Z%bool
+          then t_map1 (neg' int_width) v
+          else None.
+  Definition cmovne' (r1 r2 : bounds) : bounds
+    := let (lr1, ur1) := r1 in let (lr2, ur2) := r2 in {| lower := Z.min lr1 lr2 ; upper := Z.max ur1 ur2 |}.
+  Definition cmovne (x y r1 r2 : t) : t := t_map4 (fun _ _ => cmovne') x y r1 r2.
+  Definition cmovle' (r1 r2 : bounds) : bounds
+    := let (lr1, ur1) := r1 in let (lr2, ur2) := r2 in {| lower := Z.min lr1 lr2 ; upper := Z.max ur1 ur2 |}.
+  Definition cmovle (x y r1 r2 : t) : t := t_map4 (fun _ _ => cmovle') x y r1 r2.
+
+  Module Export Notations.
+    Delimit Scope bounds_scope with bounds.
+    Notation "b[ l ~> u ]" := {| lower := l ; upper := u |} : bounds_scope.
+    Infix "+" := add : bounds_scope.
+    Infix "-" := sub : bounds_scope.
+    Infix "*" := mul : bounds_scope.
+    Infix "<<" := shl : bounds_scope.
+    Infix ">>" := shr : bounds_scope.
+    Infix "&'" := land : bounds_scope.
+  End Notations.
+
+  Definition interp_base_type (ty : base_type) : Set := t.
+  Definition interp_op {src dst} (f : op src dst) : interp_flat_type interp_base_type src -> interp_flat_type interp_base_type dst
+    := match f in op src dst return interp_flat_type interp_base_type src -> interp_flat_type interp_base_type dst with
+       | OpConst TZ v => fun _ => SmartBuildBounds v v
+       | OpConst (TWord _) v => fun _ => SmartBuildBounds (FixedWordSizes.wordToZ v) (FixedWordSizes.wordToZ v)
+       | Add _ => fun xy => fst xy + snd xy
+       | Sub _ => fun xy => fst xy - snd xy
+       | Mul _ => fun xy => fst xy * snd xy
+       | Shl _ => fun xy => fst xy << snd xy
+       | Shr _ => fun xy => fst xy >> snd xy
+       | Land _ => fun xy => land (fst xy) (snd xy)
+       | Lor _ => fun xy => lor (fst xy) (snd xy)
+       | Neg _ int_width => fun x => neg int_width x
+       | Cmovne _ => fun xyzw => let '(x, y, z, w) := eta4 xyzw in cmovne x y z w
+       | Cmovle _ => fun xyzw => let '(x, y, z, w) := eta4 xyzw in cmovle x y z w
+       | Cast _ _ => fun x => x
+       end%bounds.
+
+  (*Definition of_wordW ty : WordW.interp_base_type ty -> interp_base_type ty
+      := match ty return WordW.interp_base_type ty -> interp_base_type ty with
+         | TZ => wordWToBounds
+         end.*)
+
+  Ltac inversion_bounds :=
+    let lower := (eval cbv [lower] in (fun x => lower x)) in
+    let upper := (eval cbv [upper] in (fun y => upper y)) in
+    repeat match goal with
+           | [ H : _ = _ :> bounds |- _ ]
+             => pose proof (f_equal lower H); pose proof (f_equal upper H); clear H;
+                cbv beta iota in *
+           | [ H : _ = _ :> t |- _ ]
+             => unfold t in H; inversion_option
+           end.
+
+  Definition bounds_to_base_type' (b : bounds) : base_type
+    := if (0 <=? lower b)%Z
+       then TWord (Z.to_nat (Z.log2_up (Z.log2_up (1 + upper b))))
+       else TZ.
+  Definition bounds_to_base_type (b : t) : base_type
+    := match b with
+       | None => TZ
+       | Some b' => bounds_to_base_type' b'
+       end.
+
+  Definition SmartCast_base {var A A'} (x : exprf base_type op (var:=var) (Tbase A))
+    : exprf base_type op (var:=var) (Tbase A')
+    := match base_type_eq_dec A A' with
+       | left pf => match pf with
+                    | eq_refl => x
+                    end
+       | right _ => Op (Cast _ A') x
+       end.
+  Definition PairCast {var A B A' B'} (x : exprf base_type op (var:=var) (Tbase A * Tbase B))
+    : exprf base_type op (var:=var) (Tbase A' * Tbase B')
+    := match x in exprf _ _ T'
+             return exprf base_type op (Tbase A' * Tbase B')%ctype
+                    -> exprf base_type op (Tbase A' * Tbase B')%ctype
+       with
+       | Pair (Tbase A0) x1 (Tbase B0) x2
+         => fun _ => Pair (SmartCast_base x1) (SmartCast_base x2)
+       | _ => fun x => x
+       end (LetIn x (fun xy => Pair (SmartCast_base (Var (fst xy))) (SmartCast_base (Var (snd xy))))).
+
+  Definition bound_op {var}
+             {src1 dst1 src2 dst2}
+             (opc1 : op src1 dst1)
+             (opc2 : op src2 dst2)
+    : forall (args2 : exprf base_type op (var:=interp_base_type) src2),
+      option
+        { new_src : flat_type base_type
+                    & exprf base_type op (var:=var) new_src
+                    -> exprf base_type op (var:=var)
+                             (SmartFlatTypeMap2
+                                (fun t v => Tbase (bounds_to_base_type v))
+                                (interpf (@interp_op) (Op opc2 args2))) }
+    := match opc1, opc2 in op src2 dst2
+             return (forall args2 : exprf base_type op (var:=interp_base_type) src2,
+                        option { new_src : _
+                                           & exprf base_type op (var:=var) new_src
+                                           -> exprf base_type op (var:=var)
+                                                    (SmartFlatTypeMap2
+                                                       (fun t v => Tbase (bounds_to_base_type v))
+                                                       (interpf (@interp_op) (@Op base_type op _ src2 dst2 opc2 args2))) })
+       with
+       | OpConst _ v, OpConst _ bs
+         => fun args2
+            => option_map
+                 (fun bounds => existT (fun new_src => exprf _ _ new_src -> _)
+                                       Unit
+                                       (fun TT => SmartCast_base (Op (OpConst v) TT)))
+                 (interpf (@interp_op) (Op (OpConst bs) args2))
+       | Add T1, Add T2 => fun _ => Some (existT _ _ (Op (Add _)))
+       | Sub T1, Sub T2 as opc2'
+         => fun args2
+            => let Targs' := (SmartFlatTypeMap2
+                                (fun t v => Tbase (bounds_to_base_type v))
+                                (interpf (@interp_op) args2)) in
+               let TR := bounds_to_base_type (interpf (@interp_op) (Op opc2' args2) (t:=Tbase _)) in
+               let Targ' : base_type
+                   := match Targs' return match Targs' with Prod (Tbase _) (Tbase _) => base_type | _ => unit end with
+                      | Prod (Tbase A) (Tbase B) => base_type_max A B
+                      | _ => tt
+                      end in
+               let T := base_type_max Targ' TR in
+               let AT := bounds_to_base_type (fst (interpf (@interp_op) args2)) in
+               let BT := bounds_to_base_type (snd (interpf (@interp_op) args2)) in
+               Some (if base_type_beq T TR
+                        return { new_src : _
+                                           & exprf base_type op new_src
+                                           -> exprf base_type op (SmartFlatTypeMap2
+                                                                    (fun t v => Tbase (bounds_to_base_type v))
+                                                                    (interpf (@interp_op) (Op opc2' args2))) }
+                     then existT _ _ (Op (Sub _))
+                     else if flat_type_beq _ base_type_beq Targs' (Tbase T * Tbase T)%ctype
+                          then existT _
+                                      (Tbase T * Tbase T)%ctype
+                                      (fun x => Op (Cast T TR) (Op (Sub T) x))
+                          else existT
+                                 (fun new_src : _
+                                  => exprf _ op new_src
+                                     -> exprf _ op (SmartFlatTypeMap2
+                                                      (fun t v => Tbase (bounds_to_base_type v))
+                                                      (interpf (@interp_op) (Op opc2' args2))))
+                                 Targs'
+                                 (fun x => Op (Cast T TR) (Op (Sub T) (PairCast (A:=AT) (B:=BT) x))))
+       | Mul T1, Mul T2 => fun _ => Some (existT _ _ (Op (Mul _)))
+       | Shl T1, Shl T2 => fun _ => Some (existT _ _ (Op (Shl _)))
+       | Shr T1, Shr T2 as opc2'
+         => fun args2
+            => let Targs' := (SmartFlatTypeMap2
+                                (fun t v => Tbase (bounds_to_base_type v))
+                                (interpf (@interp_op) args2)) in
+               let TR := bounds_to_base_type (interpf (@interp_op) (Op opc2' args2) (t:=Tbase _)) in
+               let Targ' : base_type
+                   := match Targs' return match Targs' with Prod (Tbase _) (Tbase _) => base_type | _ => unit end with
+                      | Prod (Tbase A) (Tbase B) => base_type_max A B
+                      | _ => tt
+                      end in
+               let T := base_type_max Targ' TR in
+               let AT := bounds_to_base_type (fst (interpf (@interp_op) args2)) in
+               let BT := bounds_to_base_type (snd (interpf (@interp_op) args2)) in
+               Some (if base_type_beq T TR
+                        return { new_src : _
+                                           & exprf _ op new_src
+                                           -> exprf _ op (SmartFlatTypeMap2
+                                                            (fun t v => Tbase (bounds_to_base_type v))
+                                                            (interpf (@interp_op) (Op opc2' args2))) }
+                     then existT _ _ (Op (Shr _))
+                     else if flat_type_beq _ base_type_beq Targs' (Tbase T * Tbase T)%ctype
+                          then existT _
+                                      (Tbase T * Tbase T)%ctype
+                                      (fun x => Op (Cast T TR) (Op (Shr T) x))
+                          else existT
+                                 (fun new_src : _
+                                  => exprf _ op new_src
+                                     -> exprf _ op (SmartFlatTypeMap2
+                                                      (fun t v => Tbase (bounds_to_base_type v))
+                                                      (interpf (@interp_op) (Op opc2' args2))))
+                                 Targs'
+                                 (fun x => Op (Cast T TR) (Op (Shr T) (PairCast (A:=AT) (B:=BT) x))))
+       | Land T1, Land T2 => fun _ => Some (existT _ _ (Op (Land _)))
+       | Lor T1, Lor T2 => fun _ => Some (existT _ _ (Op (Lor _)))
+       | Neg T1 int_width1, Neg T2 int_width2
+         => fun _ => if Z.eqb int_width1 int_width2
+                     then Some (existT _ _ (Op (Neg _ int_width1)))
+                     else None
+       | Cmovne T1, Cmovne T2 => fun _ => Some (existT _ _ (Op (Cmovne _)))
+       | Cmovle T1, Cmovle T2 => fun _ => Some (existT _ _ (Op (Cmovle _)))
+       | Cast A1 B1, Cast A2 B2 => fun _ => Some (existT _ _ (fun x => x))
+       | OpConst _ _, _
+       | Add _, _
+       | Sub _, _
+       | Mul _, _
+       | Shl _, _
+       | Shr _, _
+       | Land _, _
+       | Lor _, _
+       | Neg _ _, _
+       | Cmovne _, _
+       | Cmovle _, _
+       | Cast _ _, _
+         => fun _ => None
+       end.
+  Definition ZToBounds (z : Z) : bounds := {| lower := z ; upper := z |}.
+  Definition of_Z (z : Z) : t := Some (ZToBounds z).
+
+  Definition of_interp t (z : Syntax.interp_base_type t) : interp_base_type t
+    := Some (ZToBounds (match t return Syntax.interp_base_type t -> Z with
+                        | TZ => fun z => z
+                        | TWord logsz => FixedWordSizes.wordToZ
+                        end z)).
+
+  Definition MapBounds {t} (e : Expr base_type op t) input_bounds
+    : Expr
+        base_type op
+        (MapCast.new_type (fun _ => bounds_to_base_type) input_bounds
+                          (Interp (@interp_op) e))
+    := @MapInterpCastWithCastOp
+         base_type Bounds.interp_base_type
+         op (@Bounds.interp_op)
+         base_type_beq internal_base_type_dec_bl (fun _ t => Op (OpConst (ZToInterp 0)) TT)
+         (fun _ => Bounds.bounds_to_base_type)
+         (fun _ _ _ => Op (Cast _ _))
+         (fun _ _ opc => match opc with Cast _ _ => true | _ => false end)
+         (@Bounds.bound_op)
+         _ e input_bounds.
+  Definition ComputeBounds {t} (e : Expr base_type op t)
+             (input_bounds : interp_flat_type interp_base_type (domain t))
+    : interp_flat_type interp_base_type (codomain t)
+    := Interp (@interp_op) e input_bounds.
+
+  (*Definition mapf_interpToZ_T (T : flat_type base_type) : flat_type base_type
+    :=
+*)
+  Definition mapf_interpToZ {T} : interp_flat_type Syntax.interp_base_type T -> interp_flat_type (fun _ => Z) T
+    := SmartVarfMap (fun _ => interpToZ).
+
+  Fixpoint Zis_bounded_by {T1 T2} : interp_flat_type (fun _ : base_type => Z) T1 -> interp_flat_type interp_base_type T2 -> bool
+    := match T1, T2 return interp_flat_type (fun _ => Z) T1 -> interp_flat_type interp_base_type T2 -> bool with
+       | Tbase T1, Tbase T2
+         => fun val bounds
+            => match bounds with
+               | Some bounds'
+                 => (lower bounds' <=? val) && (val <=? upper bounds')
+               | None => false
+               end
+       | Unit, Unit => fun _ _ => true
+       | Prod A1 B1, Prod A2 B2
+         => fun x y => @Zis_bounded_by A1 A2 (fst x) (fst y) && @Zis_bounded_by B1 B2 (snd x) (snd y)
+       | Unit, _
+       | Tbase _, _
+       | Prod _ _, _
+         => fun _ _ => false
+       end%bool%Z.
+  Definition is_bounded_by {T1 T2} : interp_flat_type Syntax.interp_base_type T1 -> interp_flat_type interp_base_type T2 -> bool
+    := fun x y => Zis_bounded_by (mapf_interpToZ x) y.
+(*
+  Definition is_bounded_and_correct {T1 T2 TB}
+             (interpreted_val : interp_flat_type Syntax.interp_base_type T1)
+             (orig_val : interp_flat_type Syntax.interp_base_type T2)
+             (bounds : interp_flat_type interp_base_type TB)
+    : Prop
+    := mapf_interpToZ interpreted_val = orig_val
+
+  (((Tuple.map (n:=k) fe25519WToZ irop = op)
+       /\ HList.hlistP (fun v => is_bounded v = true) (Tuple.map (n:=k) fe25519WToZ irop))%type)*)
+End Bounds.
