src/Reflection/Z/Reify.v
@@ -11,19 +11,19 @@ Require Import Crypto.Reflection.LinearizeInterp.
 
 Ltac base_reify_op op op_head extra ::=
      lazymatch op_head with
-     | @Z.add => constr:(reify_op op op_head 2 Add)
-     | @Z.mul => constr:(reify_op op op_head 2 Mul)
-     | @Z.sub => constr:(reify_op op op_head 2 Sub)
-     | @Z.shiftl => constr:(reify_op op op_head 2 Shl)
-     | @Z.shiftr => constr:(reify_op op op_head 2 Shr)
-     | @Z.land => constr:(reify_op op op_head 2 Land)
-     | @Z.lor => constr:(reify_op op op_head 2 Lor)
-     | @ModularBaseSystemListZOperations.cmovne => constr:(reify_op op op_head 4 Cmovne)
-     | @ModularBaseSystemListZOperations.cmovl => constr:(reify_op op op_head 4 Cmovle)
+     | @Z.add => constr:(reify_op op op_head 2 (Add TZ))
+     | @Z.mul => constr:(reify_op op op_head 2 (Mul TZ))
+     | @Z.sub => constr:(reify_op op op_head 2 (Sub TZ))
+     | @Z.shiftl => constr:(reify_op op op_head 2 (Shl TZ))
+     | @Z.shiftr => constr:(reify_op op op_head 2 (Shr TZ))
+     | @Z.land => constr:(reify_op op op_head 2 (Land TZ))
+     | @Z.lor => constr:(reify_op op op_head 2 (Lor TZ))
+     | @ModularBaseSystemListZOperations.cmovne => constr:(reify_op op op_head 4 (Cmovne TZ))
+     | @ModularBaseSystemListZOperations.cmovl => constr:(reify_op op op_head 4 (Cmovle TZ))
      | @ModularBaseSystemListZOperations.neg
        => lazymatch extra with
           | @ModularBaseSystemListZOperations.neg ?int_width _
-            => constr:(reify_op op op_head 1 (Neg int_width))
+            => constr:(reify_op op op_head 1 (Neg TZ int_width))
           | _ => fail 100 "Anomaly: In Reflection.Z.base_reify_op: head is neg but body is wrong:" extra
           end
      end.
@@ -39,7 +39,7 @@ Ltac prove_InlineConst_Linearize_Compile_correct :=
   fun _
   => intros;
      lazymatch goal with
-     | [ |- ?R (@Syntax.Interp ?base_type_code ?interp_base_type ?op ?interp_op ?t (InlineConst ?is_const (Linearize _))) _ ]
+     | [ |- ?R (@Syntax.Interp ?base_type_code ?interp_base_type ?op ?interp_op ?t (InlineConst ?is_const (Linearize _)) ?x) _ ]
        => etransitivity;
           [ apply (@Interp_InlineConst base_type_code interp_base_type op interp_op is_const t);
             reflect_Wf base_type_eq_semidec_is_dec op_beq_bl
